theory/Bear/GroupAction.v
@@ -1,0 +1,46 @@
+Require Import TBGen.Bear.Graph.
+
+Record Group : Type := {
+  carrier : Type;
+
+  id : carrier;
+  mult : carrier -> carrier -> carrier;
+  inv : carrier -> carrier;
+
+  assoc : forall x y z, mult x (mult y z) = mult (mult x y) z;
+  id_left : forall x, mult id x = x;
+  id_right : forall x, mult x id = x;
+
+  inv_left : forall x, mult (inv x) x = id;
+  inv_right : forall x, mult x (inv x) = id;
+  }.
+
+Arguments id {_}.
+Arguments mult {_} _ _.
+Arguments inv {_} _.
+
+Infix "**" := mult (at level 10).
+
+Class GroupAction (G : Graph) (H : Group) : Type := {
+  act : carrier H -> Vert G -> Vert G;
+  act_id : forall v, act id v = v;
+  act_comp : forall v x y, act (x ** y) v = act x (act y v);
+  act_edge : forall (x : carrier H) (v v' : Vert G),
+    List.In v' (successors v) ->
+    List.In (act x v') (successors (act x v));
+  }.
+
+Arguments act {_} {_} {_} _ _.
+
+Infix "#" := act (at level 5).
+
+Lemma act_inj {G} {H} `{GroupAction G H} :
+  forall x v v', x # v = x # v' -> v = v'.
+Proof.
+  intros x v v' pf.
+  apply f_equal with (f := act (inv x)) in pf.
+  repeat rewrite <- act_comp in pf.
+  rewrite inv_left in pf.
+  repeat rewrite act_id in pf.
+  auto.
+Qed.
