theory/Bear/RomanWheelSym.v
@@ -1,0 +1,630 @@
+Require Import List.
+Import ListNotations.
+
+Require Import PrimInt63.
+Require Import Uint63.
+Require Import ZArith.
+Require Import Lia.
+
+Require Import TBGen.Util.IntHash.
+Require Import TBGen.Bear.Graph.
+Require Import TBGen.Bear.BearGame.
+Require Import TBGen.TB.TB.
+Require Import TBGen.Bear.RomanWheel.
+
+Require Import TBGen.Bear.GroupAction.
+
+Definition Fin n : Type :=
+  { i : nat | i < n }.
+
+Definition val {n} (i : Fin n) : nat :=
+  proj1_sig i.
+
+(* technically doesn't need proof irrel. *)
+Lemma val_inj {n} (i j : Fin n) :
+  val i = val j -> i = j.
+Proof.
+  destruct i as [x x_pf].
+  destruct j as [y y_pf]; simpl.
+  intro pf; subst.
+  assert (x_pf = y_pf) by
+    apply ProofIrrelevance.proof_irrelevance.
+  subst; reflexivity.
+Qed.
+
+Definition Fin_zero {n} : Fin (S n).
+Proof.
+  exists 0; lia.
+Defined.
+
+Definition Fin_plus {n} : Fin n -> Fin n -> Fin n.
+Proof.
+  intros [x x_pf] [y y_pf].
+  exists ((x + y) mod n).
+  apply Nat.mod_upper_bound; lia.
+Defined.
+
+Lemma val_plus {n} (i j : Fin n) :
+  val (Fin_plus i j) = (val i + val j) mod n.
+Proof.
+  destruct i,j; simpl.
+  reflexivity.
+Qed.
+
+Lemma Fin_plus_comm {n} (i j : Fin n) :
+  Fin_plus i j = Fin_plus j i.
+Proof.
+  apply val_inj.
+  repeat rewrite val_plus.
+  rewrite Nat.add_comm.
+  auto.
+Qed.
+
+Definition Fin_inv {n} : Fin n -> Fin n.
+Proof.
+  intros [x x_pf].
+  exists (
+    match x with
+    | 0 => 0
+    | _ => n - x
+    end).
+  destruct x; lia.
+Defined.
+
+Lemma val_inv {n} (i : Fin n) :
+  val (Fin_inv i) =
+  match val i with
+  | 0 => 0
+  | _ => n - val i
+  end.
+Proof.
+  destruct i; reflexivity.
+Qed.
+
+Lemma Fin_plus_assoc {n} (i j k : Fin n) :
+  Fin_plus i (Fin_plus j k) = Fin_plus (Fin_plus i j) k.
+Proof.
+  intros.
+  apply val_inj.
+  repeat rewrite val_plus.
+  rewrite Nat.Div0.add_mod_idemp_r.
+  rewrite Nat.Div0.add_mod_idemp_l.
+  now rewrite Nat.add_assoc.
+Qed.
+
+Lemma Fin_inv_left {n} (x : Fin (S n)) :
+  Fin_plus (Fin_inv x) x = Fin_zero.
+Proof.
+  destruct x as [x x_small].
+  apply val_inj.
+  rewrite val_plus.
+  rewrite val_inv.
+  simpl val.
+  destruct x.
+  - simpl; lia.
+  - assert (S n - S x + S x = S n) by lia.
+    rewrite H.
+    now rewrite Nat.Div0.mod_same.
+Qed.
+
+Lemma Fin_inv_right {n} (x : Fin (S n)) :
+  Fin_plus x (Fin_inv x) = Fin_zero.
+Proof.
+  - destruct x as [x x_small].
+    apply val_inj.
+    rewrite val_plus.
+    rewrite val_inv.
+    simpl val.
+    destruct x.
+    + simpl; lia.
+    + assert (S x + (S n - S x) = S n) by lia.
+      rewrite H.
+      now rewrite Nat.Div0.mod_same.
+Qed.
+
+Lemma Fin_zero_l {n} (x : Fin (S n)) :
+  Fin_plus Fin_zero x = x.
+Proof.
+  destruct x as [x x_small].
+  apply val_inj.
+  rewrite val_plus.
+  simpl val.
+  rewrite Nat.mod_small; auto.
+Qed.
+
+Lemma Fin_zero_r {n} (x : Fin (S n)) :
+  Fin_plus x Fin_zero = x.
+Proof.
+  destruct x as [x x_small].
+  apply val_inj.
+  rewrite val_plus.
+  simpl val.
+  rewrite Nat.mod_small; auto; lia.
+Qed.
+
+Definition Z_8 : Group := {|
+    carrier := Fin 8;
+    id := Fin_zero;
+    mult := Fin_plus;
+    inv := Fin_inv;
+    assoc := Fin_plus_assoc;
+    id_left := Fin_zero_l;
+    id_right := Fin_zero_r;
+    inv_left := Fin_inv_left;
+    inv_right := Fin_inv_right;
+  |}.
+
+Fixpoint rotate_spoke (n : nat) (s : Spoke) : Spoke :=
+  match n with
+  | 0 => s
+  | S m => clockwise (rotate_spoke m s)
+  end.
+
+Lemma rotate_spoke_plus (m n : nat) : forall (s : Spoke),
+  rotate_spoke (m + n) s =
+  rotate_spoke m (rotate_spoke n s).
+Proof.
+  induction m; intro.
+  - reflexivity.
+  - simpl.
+    now rewrite IHm.
+Qed.
+
+Lemma rotate_8 : forall s,
+  rotate_spoke 8 s = s.
+Proof.
+  intros []; reflexivity.
+Qed.
+
+Lemma rotate_mult_8 (n : nat) : forall (s : Spoke),
+  rotate_spoke (8 * n) s = s.
+Proof.
+  induction n; intro.
+  - reflexivity.
+  - rewrite <- mult_n_Sm.
+    rewrite rotate_spoke_plus.
+    rewrite rotate_8.
+    apply IHn.
+Qed.
+
+Lemma rotate_mod_8 (n : nat) : forall (s : Spoke),
+  rotate_spoke n s = rotate_spoke (n mod 8) s.
+Proof.
+  intro s.
+  rewrite (Nat.Div0.div_mod n 8) at 1.
+  rewrite rotate_spoke_plus.
+  now rewrite rotate_mult_8.
+Qed.
+
+Definition rotate_vert (n : nat) (v : RWVert) : RWVert :=
+  match v with
+  | Center => Center
+  | SpokeVert s l => SpokeVert (rotate_spoke n s) l
+  end.
+
+Lemma successors_Center : forall v,
+  In v (@successors RomanWheel Center) <->
+  exists s, v = SpokeVert s Mid.
+Proof.
+  intro v; split; intro pf.
+  - simpl in pf.
+    firstorder; subst; eexists; eauto.
+  - destruct pf as [s Hs]; subst.
+    simpl; destruct s; tauto.
+Qed.
+
+Lemma cw_ccw s :
+  clockwise (c_clockwise s) = s.
+Proof.
+  destruct s; auto.
+Qed.
+
+Lemma ccw_cw s :
+  c_clockwise (clockwise s) = s.
+Proof.
+  destruct s; auto.
+Qed.
+
+Lemma rotate_spoke_c_clockwise n s :
+  rotate_spoke n (c_clockwise s) =
+  c_clockwise (rotate_spoke n s).
+Proof.
+  induction n.
+  - reflexivity.
+  - simpl.
+    rewrite IHn.
+    rewrite cw_ccw.
+    now rewrite ccw_cw.
+Qed.
+
+Lemma rotate_spoke_clockwise n s :
+  rotate_spoke n (clockwise s) = 
+  clockwise (rotate_spoke n s).
+Proof.
+  induction n.
+  - reflexivity.
+  - simpl; now rewrite IHn.
+Qed.
+
+Global Instance RW_Z_8 : GroupAction RomanWheel Z_8.
+Proof.
+  refine {|
+    act := fun (x : carrier Z_8) (v : Vert RomanWheel) =>
+      rotate_vert (val x) v;
+    act_id := _;
+    act_comp := _;
+    act_edge := _;
+  |}.
+  - intros []; reflexivity.
+  - intros [] x y.
+    + reflexivity.
+    + simpl; f_equal.
+      rewrite val_plus.
+      rewrite <- rotate_mod_8.
+      now rewrite rotate_spoke_plus.
+  - intros x v v' pf.
+    destruct v.
+    + simpl rotate_vert.
+      rewrite successors_Center in *.
+      destruct pf as [s Hs]; subst.
+      exists (rotate_spoke (val x) s).
+      reflexivity.
+    + simpl successors in *.
+      destruct l.
+      * destruct pf as [pf1|[pf2|[pf3|[]]]]; subst.
+        -- now left.
+        -- right; now left.
+        -- right; right; now left.
+      * destruct pf as [pf1|[pf2|[pf3|[]]]]; subst.
+        -- now left.
+        -- right; now left.
+        -- right; right; left; simpl.
+           now rewrite rotate_spoke_c_clockwise.
+      * destruct pf as [pf1|[pf2|[pf3|[]]]]; subst.
+        -- now left.
+        -- right; now left.
+        -- right; right; left; simpl.
+           simpl.
+           now rewrite rotate_spoke_clockwise.
+Defined.
+
+Definition spoke_nat (s : Spoke) : nat :=
+  match s with
+  | S1 => 0
+  | S2 => 7
+  | S3 => 6
+  | S4 => 5
+  | S5 => 4
+  | S6 => 3
+  | S7 => 2
+  | S8 => 1
+  end.
+
+Lemma spoke_nat_small s : spoke_nat s < 8.
+Proof.
+  destruct s; simpl; lia.
+Qed.
+
+Definition spoke_Fin (s : Spoke) : Fin 8 :=
+  exist _ (spoke_nat s) (spoke_nat_small s).
+
+Fixpoint mult {n} (k : nat) (i : Fin (S n)) : Fin (S n) :=
+  match k with
+  | 0 => Fin_zero
+  | S m => Fin_plus i (mult m i)
+  end.
+
+Fixpoint spoke_total (vs : list RWVert) : carrier Z_8 :=
+  match vs with
+  | [] => Fin_zero
+  | Center :: vs' => spoke_total vs'
+  | SpokeVert s _ :: vs' => Fin_plus (spoke_Fin s) (spoke_total vs')
+  end.
+
+Definition one : carrier Z_8.
+Proof.
+  exists 1; lia.
+Defined.
+
+Definition compute_rotation (s : BG_State RomanWheel) : carrier Z_8 :=
+  match bear s with
+  | Center => mult 3 (spoke_total (hunters s))
+  | SpokeVert s' l => spoke_Fin s'
+  end.
+
+Lemma spoke_Fin_clockwise : forall s,
+  spoke_Fin (clockwise s) =
+  Fin_plus (inv one) (spoke_Fin s).
+Proof.
+  intro s.
+  apply val_inj.
+  destruct s; reflexivity.
+Qed.
+
+Lemma spoke_Fin_rotate_spoke_nat : forall n s,
+  spoke_Fin (rotate_spoke n s) =
+  Fin_plus (mult n (inv one)) (spoke_Fin s).
+Proof.
+  induction n; intro s.
+  - simpl rotate_spoke.
+    simpl mult.
+    symmetry; apply (@id_left Z_8).
+  - simpl rotate_spoke.
+    rewrite spoke_Fin_clockwise.
+    unfold mult; fold @mult.
+    rewrite IHn.
+    apply (@assoc Z_8).
+Qed.
+
+Lemma val_mult n (x : carrier Z_8) :
+  val (mult n x) = (n * val x) mod 8.
+Proof.
+  induction n.
+  - reflexivity.
+  - simpl mult.
+    rewrite val_plus.
+    simpl Nat.mul.
+    rewrite IHn.
+    now rewrite Nat.Div0.add_mod_idemp_r.
+Qed.
+
+Lemma val_one : val one = 1.
+Proof.
+  reflexivity.
+Qed.
+
+Lemma spoke_Fin_rotate_spoke : forall (x : carrier Z_8) s,
+  spoke_Fin (rotate_spoke (val x) s) =
+  (inv x) ** (spoke_Fin s).
+Proof.
+  intros x s; simpl.
+  rewrite spoke_Fin_rotate_spoke_nat.
+  f_equal.
+  apply val_inj.
+  rewrite val_inv.
+  rewrite val_mult.
+  unfold inv.
+  unfold Z_8.
+  rewrite val_inv.
+  rewrite val_one.
+  destruct x as [x x_pf].
+  simpl val.
+  destruct x.
+  - reflexivity.
+  - destruct x; [reflexivity|].
+    destruct x; [reflexivity|].
+    destruct x; [reflexivity|].
+    destruct x; [reflexivity|].
+    destruct x; [reflexivity|].
+    destruct x; [reflexivity|].
+    destruct x; [reflexivity|].
+    destruct x; [reflexivity|].
+    lia.
+Defined.
+
+Lemma spoke_total_insert_Center
+  (xs : list (Vert RomanWheel)) :
+  spoke_total (Sort.insert (Center : Vert RomanWheel) xs) =
+  spoke_total xs.
+Proof.
+  induction xs.
+  - reflexivity.
+  - unfold Sort.insert; fold @Sort.insert.
+    destruct Sort.ord_le_dec.
+    + reflexivity.
+    + unfold spoke_total; fold @spoke_total.
+      rewrite IHxs; reflexivity.
+Qed.
+
+Lemma spoke_total_insert_spoke
+  (xs : list (Vert RomanWheel)) s l :
+  spoke_total (Sort.insert (SpokeVert s l : Vert RomanWheel) xs) =
+  Fin_plus (spoke_Fin s) (spoke_total xs).
+Proof.
+  induction xs.
+  - reflexivity.
+  - unfold Sort.insert; fold @Sort.insert.
+    destruct Sort.ord_le_dec.
+    + reflexivity.
+    + unfold spoke_total; fold @spoke_total.
+      rewrite IHxs.
+      destruct a; auto.
+      rewrite Fin_plus_assoc.
+      rewrite (Fin_plus_comm (spoke_Fin s0)).
+      now rewrite <- Fin_plus_assoc.
+Qed.
+
+Lemma spoke_total_insertion_sort (xs : list (Vert RomanWheel)) :
+  spoke_total (Sort.insertion_sort xs) = spoke_total xs.
+Proof.
+  induction xs.
+  - reflexivity.
+  - simpl Sort.insertion_sort.
+    destruct a.
+    + simpl spoke_total.
+      now rewrite spoke_total_insert_Center.
+    + unfold spoke_total at 2.
+      fold @spoke_total.
+      rewrite <- IHxs.
+      now rewrite spoke_total_insert_spoke.
+Qed.
+
+Lemma spoke_total_map_rotate_vert n (xs : list (Vert RomanWheel)) :
+  (~ In Center xs) ->
+  spoke_total (map (rotate_vert n) xs) =
+  Fin_plus (mult (length xs) (mult n (inv one))) (spoke_total xs).
+Proof.
+  intro pf.
+  induction xs.
+  - apply val_inj; reflexivity.
+  - simpl map.
+    unfold spoke_total; fold spoke_total.
+    destruct a.
+    + elim pf; now left.
+    + simpl rotate_vert.
+      rewrite IHxs.
+      * simpl length.
+        rewrite spoke_Fin_rotate_spoke_nat.
+        pose (a := spoke_total xs); fold a.
+        pose (b := mult n (inv one)); fold b.
+        simpl mult.
+        pose (c := spoke_Fin s); fold c.
+        pose (d := mult (length xs) b); simpl Vert in d.
+        fold d.
+        rewrite <- Fin_plus_assoc.
+        rewrite (Fin_plus_assoc c d a).
+        rewrite (Fin_plus_comm c d).
+        rewrite <- (Fin_plus_assoc d c a).
+        now rewrite Fin_plus_assoc.
+      * intro; apply pf; now right.
+Qed.
+
+Lemma mult_Fin_plus k (x y : carrier Z_8) :
+  mult k (Fin_plus x y) =
+  Fin_plus (mult k x) (mult k y).
+Proof.
+  apply val_inj.
+  rewrite val_plus.
+  rewrite val_mult.
+  rewrite val_plus.
+  repeat rewrite val_mult.
+  do 2 rewrite Nat.Div0.add_mod.
+  destruct x as [x ?].
+  destruct y as [y ?].
+  simpl val.
+  repeat rewrite (Nat.mod_small x); auto.
+  repeat rewrite (Nat.mod_small y); auto.
+  rewrite Nat.Div0.mul_mod_idemp_r.
+  rewrite Nat.mul_add_distr_l.
+  now rewrite Nat.Div0.add_mod.
+Qed.
+
+Lemma Fin_plus_l_cancel {n} (x y z : Fin (S n)) :
+  Fin_plus x y = Fin_plus x z ->
+  y = z.
+Proof.
+  intro pf.
+  rewrite <- (Fin_zero_l y).
+  rewrite <- (Fin_inv_left x).
+  rewrite <- Fin_plus_assoc.
+  rewrite pf.
+  rewrite Fin_plus_assoc.
+  rewrite Fin_inv_left.
+  apply Fin_zero_l.
+Qed.
+
+Lemma Fin_inv_plus (x y : carrier Z_8) :
+  Fin_inv (Fin_plus x y) =
+  Fin_plus (Fin_inv y) (Fin_inv x).
+Proof.
+  apply (Fin_plus_l_cancel (Fin_plus x y)).
+  rewrite Fin_inv_right.
+  rewrite Fin_plus_assoc.
+  rewrite <- (Fin_plus_assoc x).
+  rewrite Fin_inv_right.
+  rewrite Fin_zero_r.
+  now rewrite Fin_inv_right.
+Qed.
+
+Lemma mult_add k l (x : carrier Z_8) :
+  mult (k + l) x =
+  Fin_plus (mult k x) (mult l x).
+Proof.
+  induction k.
+  - simpl mult.
+    symmetry; apply (@id_left Z_8).
+  - simpl.
+    rewrite IHk.
+    apply (@assoc Z_8).
+Qed.
+
+Lemma mult_comp k l (x : carrier Z_8) :
+  mult k (mult l x) = mult (k * l) x.
+Proof.
+  induction k.
+  - reflexivity.
+  - simpl.
+    rewrite IHk.
+    now rewrite mult_add.
+Qed.
+
+Lemma mult_inv k (x : carrier Z_8) :
+  mult k (Fin_inv x) = Fin_inv (mult k x).
+Proof.
+  induction k.
+  - simpl mult.
+    now apply val_inj.
+  - simpl mult.
+    rewrite IHk.
+    rewrite Fin_plus_comm.
+    now rewrite Fin_inv_plus.
+Qed.
+
+Lemma compute_rotation_BG_State_act : forall (x : carrier Z_8) s,
+  compute_rotation (BG_State_act x s) =
+  compute_rotation s ** (inv x).
+Proof.
+  intros.
+  destruct (bear s) eqn:?.
+  - unfold compute_rotation.
+    simpl bear.
+    rewrite Heqv.
+    simpl rotate_vert.
+    cbv iota.
+    simpl hunters.
+    rewrite spoke_total_insertion_sort.
+    rewrite spoke_total_map_rotate_vert.
+    + rewrite hunters_3.
+      pose (y := spoke_total (hunters s)).
+      fold y.
+      rewrite mult_Fin_plus.
+      rewrite Fin_plus_comm.
+      unfold GroupAction.mult.
+      unfold Z_8.
+      f_equal.
+      repeat rewrite mult_comp.
+      unfold inv.
+      rewrite mult_inv.
+      f_equal.
+      apply val_inj.
+      rewrite val_mult.
+      rewrite Nat.Div0.mul_mod.
+      rewrite val_one.
+      rewrite (Nat.Div0.mul_mod (3 * 3)).
+      simpl ((3 * 3) mod 8).
+      simpl (1 mod 8).
+      rewrite Nat.mul_1_l.
+      rewrite Nat.mul_1_r.
+      repeat rewrite Nat.Div0.mod_mod.
+      apply Nat.mod_small.
+      destruct x; simpl; auto.
+    + rewrite <- Heqv.
+      apply s.
+  - unfold compute_rotation.
+    simpl.
+    rewrite Heqv.
+    simpl rotate_vert.
+    cbv iota.
+    rewrite spoke_Fin_rotate_spoke.
+    rewrite Fin_plus_comm.
+    reflexivity.
+Qed.
+
+Global Instance RW_OrbitSelector : OrbitSelector RomanWheel Z_8.
+Proof.
+  refine {|
+    select := fun s => BG_State_act (compute_rotation s) s
+  |}.
+  - intro s.
+    exists (compute_rotation s).
+    reflexivity.
+  - intros s x.
+    rewrite compute_rotation_BG_State_act.
+    rewrite BG_State_act_comp.
+    rewrite <- (BG_State_act_comp (inv x)).
+    rewrite inv_left.
+    now rewrite BG_State_act_id.
+Defined.
+
+Definition RW_TB :=
+  Bear_TB RomanWheel Z_8.
